restructuring

cedar-dafny/def/util.dfy
@@ -29,9 +29,9 @@ module def.util {
   ghost predicate IsTotalOrder<A(!new)>(R: (A, A) -> bool) {
     // connexity
     && (forall a, b :: R(a, b) || R(b, a))
-    // antisymmetry
+       // antisymmetry
     && (forall a, b | R(a, b) && R(b, a) :: a == b)
-    // transitivity
+       // transitivity
     && (forall a, b, c | R(a, b) && R(b, c) :: R(a, c))
   }
 
@@ -205,5 +205,21 @@ module def.util {
     assert IsTotalOrder(PathLeq) by {
       SeqLeqIsTotalOrder(PathLeq, IdLeq);
     }
+  }
+
+  // KeyExists and LastOfKey are helpers about association lists that are used in
+  // validation.dfy, so we lift them here.
+  // We use these as an abbreviation for the quantifier alternation:
+  // exists i :: 0 <= i < |es| && (forall j :: i < j < |es| => ...)
+  // This helps dafny prove some of our lemmas about record evaluation and validation.
+  ghost predicate KeyExists<K,V>(k: K, es: seq<(K,V)>) {
+    exists i :: 0 <= i < |es| && es[i].0 == k
+  }
+
+  opaque ghost function LastOfKey<K,V>(k: K, es: seq<(K,V)>): (res: V)
+    requires KeyExists(k,es)
+    ensures exists i :: 0 <= i < |es| && es[i].0 == k && es[i].1 == res && (forall j | i < j < |es| :: es[j].0 != k)
+  {
+    if (es[0].0 == k && (forall j | 0 < j < |es| :: es[j].0 != k)) then es[0].1 else LastOfKey(k,es[1..])
   }
 }
