cedar-dafny/thm/eval/basic.dfy
@@ -1,0 +1,59 @@
+/*
+ * Copyright 2022-2023 Amazon.com, Inc. or its affiliates. All Rights Reserved.
+ *
+ * Licensed under the Apache License, Version 2.0 (the "License");
+ * you may not use this file except in compliance with the License.
+ * You may obtain a copy of the License at
+ *
+ *      https://www.apache.org/licenses/LICENSE-2.0
+ *
+ * Unless required by applicable law or agreed to in writing, software
+ * distributed under the License is distributed on an "AS IS" BASIS,
+ * WITHOUT WARRANTIES OR CONDITIONS OF ANY KIND, either express or implied.
+ * See the License for the specific language governing permissions and
+ * limitations under the License.
+ */
+
+include "../../def/all.dfy"
+
+module eval.basic {
+  import opened def.base
+  import opened def.core
+  import opened def.engine
+  import opened def.util
+
+  lemma EntityInOrEqEntitySemantics(x1: Expr, e1: EntityUID, x2: Expr, e2: EntityUID, eval: Evaluator)
+    requires eval.interpret(x1) == Ok(Value.EntityUID(e1))
+    requires eval.interpret(x2) == Ok(Value.EntityUID(e2))
+    requires
+      eval.interpret(BinaryApp(BinaryOp.In, x1, x2)) == Ok(Value.TRUE) ||
+      eval.interpret(BinaryApp(BinaryOp.Eq, x1, x2)) == Ok(Value.TRUE)
+    ensures eval.entityInEntity(e1, e2)
+  { }
+
+  lemma AndSemantics(e1: Expr, e2: Expr, eval: Evaluator)
+    requires eval.interpret(And(e1, e2)) == Ok(Value.TRUE)
+    ensures eval.interpret(e1) == Ok(Value.TRUE)
+    ensures eval.interpret(e2) == Ok(Value.TRUE)
+  { }
+
+  lemma InterpretRecordLemmaOk(es: seq<(Attr,Expr)>, E: Evaluator)
+    requires E.interpretRecord(es).Ok?
+    ensures forall i :: 0 <= i < |es| ==> es[i].0 in E.interpretRecord(es).value.Keys && E.interpret(es[i].1).Ok?
+    ensures forall k | k in E.interpretRecord(es).value.Keys :: KeyExists(k,es) && E.interpret(LastOfKey(k,es)) == base.Ok(E.interpretRecord(es).value[k])
+  {}
+
+  lemma InterpretRecordLemmaErr(es: seq<(Attr,Expr)>, E: Evaluator)
+    requires E.interpretRecord(es).Err?
+    ensures exists i :: 0 <= i < |es| && E.interpret(es[i].1) == base.Err(E.interpretRecord(es).error) && (forall j | 0 <= j < i :: E.interpret(es[j].1).Ok?)
+  {}
+
+  lemma InterpretSetLemma(es: seq<Expr>, E: Evaluator)
+    ensures E.interpretSet(es).Ok? ==> forall v | v in E.interpretSet(es).value :: exists i :: 0 <= i < |es| && E.interpret(es[i]) == base.Ok(v)
+    ensures (forall e | e in es :: E.interpret(e).Ok?) ==> E.interpretSet(es).Ok?
+    ensures (exists i :: 0 <= i < |es| && E.interpret(es[i]).Err?) ==> E.interpretSet(es).Err?
+    ensures E.interpretSet(es).Err? <==> exists i :: 0 <= i < |es| && E.interpret(es[i]).Err? && (forall j | 0 <= j < i :: E.interpret(es[j]).Ok?);
+    ensures E.interpretSet(es).Err? ==> exists i :: 0 <= i < |es| && E.interpret(es[i]).Err? && E.interpret(es[i]).error == E.interpretSet(es).error && (forall j | 0 <= j < i :: E.interpret(es[j]).Ok?);
+  {}
+
+}
